src/basic/const.fs
@@ -17,4 +17,4 @@ type sconst =
   | Const_string      of array<byte> * Range.range           (* unicode encoded, F#/Caml independent *)
   | Const_range       of Range.range                         (* not denotable by the programmer *)
   | Const_reify                                              (* a coercion from a computation to a Tot term *)
-  | Const_reflect                                            (* a coercion from a Tot term to a computation *)
+  | Const_reflect     of Ident.lid                           (* a coercion from a Tot term to an l-computation type *)
