examples/dm4free/natST.fst
@@ -119,7 +119,15 @@ let f (_:unit) : St unit =
     let _, n1 = reify (incr2 ()) n0 in
     (* assert (n1 = n0 + 1); *)
     put n1
-    
+
+let g (_:unit) : St unit =
+    let n0 = get () in
+    let f : st_repr unit (fun n0 post -> post ((), n0 + 2)) =
+      fun n0 -> (), n0+2 in 
+    STATE.reflect f;
+    let n1 = get () in 
+    assert (n0 + 2 = n1)
+
 (* sub_effect PURE ~> STATE { *)
 (*   lift_wp: #a:Type -> #wp:pure_wp a -> st_wp a = ... *)
 (*   lift   : #a:Type -> #wp:pure_wp a -> f:PURE.repr a wp -> STATE.repr a (lift_star wp) = ... *)
